Wrote up Chaining

09ChainedEnvironment/Chaining.thy
@@ -2,101 +2,163 @@ theory Chaining
   imports ChainedEnvironment "../08HeapMemory/HeapMemory"
 begin
 
-section \<open>Converting environments to chained form \<close>
+section \<open>Chaining environments\<close>
 
-abbreviation chain_structured :: "closure\<^sub>v heap \<Rightarrow> (ptr \<times> ptr) heap \<Rightarrow> bool" where
-  "chain_structured h env \<equiv> heap_all (\<lambda>p (v, p'). p' \<le> p \<and> hcontains h v) env"
+text \<open>Restoring environments from linked-list form is a matter of following the pointers down until 
+we reach the end. To ensure termination, we only follow pointers to lower in the heap - but since we 
+allocate in linear order, this means earlier in the heap, and of course, just as with the value 
+stack, each environment can only build on preexisting ones; so we will never encounter a pointer to 
+higher up.\<close>
 
-primrec chained_stack_pointer :: "(ptr \<times> ptr) heap \<Rightarrow> ptr \<Rightarrow> bool" where
-  "chained_stack_pointer env 0 = True"
-| "chained_stack_pointer env (Suc p) = hcontains env p"
+fun unchain_env :: "('a \<times> ptr) heap \<Rightarrow> ptr \<Rightarrow> 'a list" where
+  "unchain_env \<Delta> 0 = []"
+| "unchain_env \<Delta> (Suc p) = (case hlookup \<Delta> p of 
+      (v, p') \<Rightarrow> v # (if p' \<le> p then unchain_env \<Delta> p' else undefined))"
 
-primrec chained_frame :: "(ptr \<times> ptr) heap \<Rightarrow> (ptr \<times> nat) \<Rightarrow> bool" where
-  "chained_frame env (p, pc) = chained_stack_pointer env p"
-
-abbreviation chained_stack :: "(ptr \<times> ptr) heap \<Rightarrow> (ptr \<times> nat) list \<Rightarrow> bool" where
-  "chained_stack env sfs \<equiv> list_all (chained_frame env) sfs"
-
-abbreviation chained_vals :: "closure\<^sub>v heap \<Rightarrow> ptr list \<Rightarrow> bool" where
-  "chained_vals h vs \<equiv> list_all (hcontains h) vs"
-
-primrec chained_closure :: "(ptr \<times> ptr) heap \<Rightarrow> closure\<^sub>v \<Rightarrow> bool" where
-  "chained_closure env (Const\<^sub>v n) = True"
-| "chained_closure env (Lam\<^sub>v p pc) = chained_frame env (p, pc)"
-
-abbreviation chained_closures :: "(ptr \<times> ptr) heap \<Rightarrow> closure\<^sub>v heap \<Rightarrow> bool" where
-  "chained_closures env h \<equiv> heap_all (\<lambda>p. chained_closure env) h"
-
-primrec chained_state :: "state\<^sub>v \<Rightarrow> bool" where
-  "chained_state (S\<^sub>v h env vs sfs) = (
-    chain_structured h env \<and> chained_closures env h \<and> chained_vals h vs \<and> chained_stack env sfs)"
-
-fun unstack_list :: "(ptr \<times> ptr) heap \<Rightarrow> ptr \<Rightarrow> ptr list" where
-  "unstack_list env 0 = []"
-| "unstack_list env (Suc p) = (case hlookup env p of 
-      (v, p') \<Rightarrow> v # (if p' \<le> p then unstack_list env p' else undefined))"
+text \<open>We map the transformation through the whole evaluation state.\<close>
 
 primrec unchain_closure :: "(ptr \<times> ptr) heap \<Rightarrow> closure\<^sub>v \<Rightarrow> closure\<^sub>h" where
-  "unchain_closure env (Const\<^sub>v k) = Const\<^sub>h k"
-| "unchain_closure env (Lam\<^sub>v p pc) = Lam\<^sub>h (unstack_list env p) pc"
+  "unchain_closure \<Delta> (Const\<^sub>v n) = Const\<^sub>h n"
+| "unchain_closure \<Delta> (Lam\<^sub>v p\<^sub>\<Delta> p\<^sub>\<C>) = Lam\<^sub>h (unchain_env \<Delta> p\<^sub>\<Delta>) p\<^sub>\<C>"
 
-definition unchain_heap :: "closure\<^sub>v heap \<Rightarrow> (ptr \<times> ptr) heap \<Rightarrow> closure\<^sub>h heap" where
-  "unchain_heap h env = hmap (unchain_closure env) h"
+abbreviation unchain_heap :: "closure\<^sub>v heap \<Rightarrow> (ptr \<times> ptr) heap \<Rightarrow> closure\<^sub>h heap" where
+  "unchain_heap h \<Delta> \<equiv> hmap (unchain_closure \<Delta>) h"
 
 primrec unchain_frame :: "(ptr \<times> ptr) heap \<Rightarrow> (ptr \<times> nat) \<Rightarrow> (ptr list \<times> nat)" where
-  "unchain_frame env (p, pc) = (unstack_list env p, pc)"
+  "unchain_frame \<Delta> (p\<^sub>\<Delta>, p\<^sub>\<C>) = (unchain_env \<Delta> p\<^sub>\<Delta>, p\<^sub>\<C>)"
 
-definition unchain_stack :: "(ptr \<times> ptr) heap \<Rightarrow> (ptr \<times> nat) list \<Rightarrow> (ptr list \<times> nat) list" where
-  "unchain_stack env sfs = map (unchain_frame env) sfs"
+abbreviation unchain_stack :: "(ptr \<times> ptr) heap \<Rightarrow> (ptr \<times> nat) list \<Rightarrow> (ptr list \<times> nat) list" where
+  "unchain_stack \<Delta> s \<equiv> map (unchain_frame \<Delta>) s"
 
 primrec unchain_state :: "state\<^sub>v \<Rightarrow> state\<^sub>h" where
-  "unchain_state (S\<^sub>v h env vs sfs) = S\<^sub>h (unchain_heap h env) vs (unchain_stack env sfs)"
+  "unchain_state (S\<^sub>v h \<Delta> \<V> s) = S\<^sub>h (unchain_heap h \<Delta>) \<V> (unchain_stack \<Delta> s)"
 
-lemma [simp]: "chain_structured h env \<Longrightarrow> 
-  heap_all (\<lambda>p (y, p'). p' \<le> p \<and> (y = x \<or> hcontains h y)) env"
+lemma halloc_unchain_heap_const [simp]: "halloc h (Const\<^sub>v n) = (h', p) \<Longrightarrow> 
+  halloc (unchain_heap h \<Delta>) (Const\<^sub>h n) = (unchain_heap h' \<Delta>, p)"
 proof -
-  have "\<And>a b. (\<lambda>p (v, p'). p' \<le> p \<and> hcontains h v) a b \<Longrightarrow> 
-    (\<lambda>p (y, p'). p' \<le> p \<and> (y = x \<or> hcontains h y)) a b" by (simp split: prod.splits)
-  moreover assume "chain_structured h env"
-  ultimately show "heap_all (\<lambda>p (y, p'). p' \<le> p \<and> (y = x \<or> hcontains h y)) env" 
-    by (rule heap_all_implication)
+  assume "halloc h (Const\<^sub>v n) = (h', p)"
+  hence "halloc (hmap (unchain_closure \<Delta>) h) (unchain_closure \<Delta> (Const\<^sub>v n)) = 
+    (hmap (unchain_closure \<Delta>) h', p)" by (metis halloc_map)
+  thus ?thesis by simp
 qed
 
-lemma [simp]: "unchain_heap hempty env = hempty"
-  by (simp add: unchain_heap_def)
+lemma halloc_unchain_heap_lam [simp]: "halloc h (Lam\<^sub>v p\<^sub>\<Delta> p\<^sub>\<C>) = (h', v) \<Longrightarrow> 
+  halloc (unchain_heap h \<Delta>) (Lam\<^sub>h (unchain_env \<Delta> p\<^sub>\<Delta>) p\<^sub>\<C>) = (unchain_heap h' \<Delta>, v)"
+proof -
+  assume "halloc h (Lam\<^sub>v p\<^sub>\<Delta> p\<^sub>\<C>) = (h', v)"
+  hence "halloc (hmap (unchain_closure \<Delta>) h) (unchain_closure \<Delta> (Lam\<^sub>v p\<^sub>\<Delta> p\<^sub>\<C>)) = 
+    (hmap (unchain_closure \<Delta>) h', v)" by (metis halloc_map)
+  thus ?thesis by simp
+qed
 
-lemma [elim]: "hcontains env p \<Longrightarrow> p' \<le> p \<Longrightarrow> chained_stack_pointer env p'"
-proof (induction p')
-  case (Suc p')
-  thus ?case by auto
-qed simp_all
+text \<open>We define a set of predicates to verify our "no upward pointers" condition.\<close>
 
-lemma [elim]: "chained_stack_pointer env p \<Longrightarrow> p' \<le> p \<Longrightarrow> chained_stack_pointer env p'"
-proof (induction p')
-  case (Suc p')
-  thus ?case by (cases p) auto
-qed simp_all
+abbreviation chain_structured :: "closure\<^sub>v heap \<Rightarrow> (ptr \<times> ptr) heap \<Rightarrow> bool" where
+  "chain_structured h \<Delta> \<equiv> heap_all (\<lambda>p (v, p'). p' \<le> p \<and> hcontains h v) \<Delta>"
 
-lemma [simp]: "chain_structured h env \<Longrightarrow> chained_stack_pointer env p \<Longrightarrow> 
-  halloc env a = (env', b) \<Longrightarrow> unstack_list env' p = unstack_list env p" 
-proof (induction env p rule: unstack_list.induct)
-  case (2 env p)
-  obtain v p' where V: "hlookup env p = (v, p')" by (cases "hlookup env p")
-  from 2 have H: "hcontains env p" by auto
+primrec chained_heap_pointer :: "(ptr \<times> ptr) heap \<Rightarrow> ptr \<Rightarrow> bool" where
+  "chained_heap_pointer \<Delta> 0 = True"
+| "chained_heap_pointer \<Delta> (Suc p) = hcontains \<Delta> p"
+
+primrec chained_frame :: "(ptr \<times> ptr) heap \<Rightarrow> (ptr \<times> nat) \<Rightarrow> bool" where
+  "chained_frame \<Delta> (p\<^sub>\<Delta>, p\<^sub>\<C>) = chained_heap_pointer \<Delta> p\<^sub>\<Delta>"
+
+abbreviation chained_stack :: "(ptr \<times> ptr) heap \<Rightarrow> (ptr \<times> nat) list \<Rightarrow> bool" where
+  "chained_stack \<Delta> s \<equiv> list_all (chained_frame \<Delta>) s"
+
+abbreviation chained_vals :: "closure\<^sub>v heap \<Rightarrow> ptr list \<Rightarrow> bool" where
+  "chained_vals h \<V> \<equiv> list_all (hcontains h) \<V>"
+
+primrec chained_closure :: "(ptr \<times> ptr) heap \<Rightarrow> closure\<^sub>v \<Rightarrow> bool" where
+  "chained_closure \<Delta> (Const\<^sub>v n) = True"
+| "chained_closure \<Delta> (Lam\<^sub>v p\<^sub>\<Delta> p\<^sub>\<C>) = chained_heap_pointer \<Delta> p\<^sub>\<Delta>"
+
+abbreviation chained_closures :: "(ptr \<times> ptr) heap \<Rightarrow> closure\<^sub>v heap \<Rightarrow> bool" where
+  "chained_closures \<Delta> h \<equiv> heap_all (\<lambda>p. chained_closure \<Delta>) h"
+
+primrec chained_state :: "state\<^sub>v \<Rightarrow> bool" where
+  "chained_state (S\<^sub>v h \<Delta> \<V> s) = (
+    chain_structured h \<Delta> \<and> chained_closures \<Delta> h \<and> chained_vals h \<V> \<and> chained_stack \<Delta> s)"
+
+lemma chained_heap_pointer_unfold [elim]: "hcontains \<Delta> p \<Longrightarrow> p' \<le> p \<Longrightarrow> chained_heap_pointer \<Delta> p'"
+  by (induction p') auto
+
+lemma lookup_unchain_env [simp]: "chain_structured h \<Delta> \<Longrightarrow> chained_heap_pointer \<Delta> p \<Longrightarrow>
+  lookup (unchain_env \<Delta> p) x = chain_lookup \<Delta> p x"
+proof (induction \<Delta> p x rule: chain_lookup.induct)
+  case (3 \<Delta> p x)
+  obtain v p' where V: "hlookup \<Delta> p = (v, p')" by (cases "hlookup \<Delta> p")
+  from 3 have "hcontains \<Delta> p" by auto
+  with 3 V have P: "p' \<le> p" using hlookup_all by fast
+  with 3 V have "chained_heap_pointer \<Delta> p'" by auto
+  with 3(1, 2) V P show ?case by fastforce
+qed (simp_all split: prod.splits)
+
+lemma halloc_unchain_env [simp]: "chain_structured h \<Delta> \<Longrightarrow> chained_heap_pointer \<Delta> p \<Longrightarrow> 
+  halloc \<Delta> a = (\<Delta>', b) \<Longrightarrow> unchain_env \<Delta>' p = unchain_env \<Delta> p" 
+proof (induction \<Delta> p rule: unchain_env.induct)
+  case (2 \<Delta> p)
+  obtain v p' where V: "hlookup \<Delta> p = (v, p')" by (cases "hlookup \<Delta> p")
+  from 2 have H: "hcontains \<Delta> p" by auto
   with 2 V have P: "p' \<le> p" using hlookup_all by fast
-  with 2 have "chained_stack_pointer env p'" by auto
-  with 2 V P have U: "unstack_list env' p' = unstack_list env p'" by simp
-  from 2 V H have "hlookup env' p = (v, p')" by simp
+  with 2 have "chained_heap_pointer \<Delta> p'" by auto
+  with 2 V P have U: "unchain_env \<Delta>' p' = unchain_env \<Delta> p'" by simp
+  from 2 V H have "hlookup \<Delta>' p = (v, p')" by simp
   with V P U show ?case by simp
 qed simp_all
 
-lemma unfold_unstack_list [simp]: "chain_structured h env \<Longrightarrow> chained_stack_pointer env p \<Longrightarrow> 
-  halloc env (v, p) = (env', p') \<Longrightarrow> unstack_list env' (Suc p') = v # unstack_list env p"
+lemma halloc_unchain_env2 [elim]: "hcontains \<Delta> p \<Longrightarrow> halloc \<Delta> v = (\<Delta>', q) \<Longrightarrow> 
+  unchain_env \<Delta>' p = unchain_env \<Delta> p"
+proof (induction \<Delta> p rule: unchain_env.induct)
+  case (2 \<Delta> p)
+  obtain vv p' where V: "hlookup \<Delta> p = (vv, p')" by (cases "hlookup \<Delta> p")
+  from 2(2) have "hcontains \<Delta> p" by fast
+  with 2(3) V have V': "hlookup \<Delta>' p = (vv, p')" by simp
+  from 2(2) V have "p' \<le> p \<Longrightarrow> hcontains \<Delta> p'" by auto
+  with 2 V have "p' \<le> p \<Longrightarrow> unchain_env \<Delta>' p' = unchain_env \<Delta> p'" by metis
+  with V V' show ?case by simp
+qed simp_all
+
+lemma halloc_unchain_env3 [elim]: "chained_heap_pointer \<Delta> a \<Longrightarrow> halloc \<Delta> v = (\<Delta>', p) \<Longrightarrow> 
+  unchain_env \<Delta>' a = unchain_env \<Delta> a"
+proof (induction a)
+  case (Suc p)
+  moreover obtain v' p' where "hlookup \<Delta> p = (v', p')" by (cases "hlookup \<Delta> p")
+  moreover from Suc have "p' \<le> p \<Longrightarrow> hcontains \<Delta> p'" by auto
+  ultimately show ?case by auto
+qed simp_all
+
+lemma halloc_unchain_heap [elim]: "chain_structured h \<Delta> \<Longrightarrow> chained_closures \<Delta> h \<Longrightarrow> 
+  halloc \<Delta> v = (\<Delta>', p) \<Longrightarrow> unchain_heap h \<Delta>' = unchain_heap h \<Delta>"
 proof -
-  assume A: "chain_structured h env"
-  assume B: "chained_stack_pointer env p"
-  assume C: "halloc env (v, p) = (env', p')"
-  moreover with A B have "unstack_list env' p = unstack_list env p" by simp
+  assume S: "chain_structured h \<Delta>" and C: "chained_closures \<Delta> h" 
+    and A: "halloc \<Delta> v = (\<Delta>', p)"
+  have "\<And>x. hcontains h x \<Longrightarrow> unchain_closure \<Delta>' (hlookup h x) = 
+    unchain_closure \<Delta> (hlookup h x)" 
+  proof -
+    fix x
+    assume X: "hcontains h x"
+    show "unchain_closure \<Delta>' (hlookup h x) = unchain_closure \<Delta> (hlookup h x)" 
+    proof (cases "hlookup h x")
+      case (Lam\<^sub>v p\<^sub>\<Delta> p\<^sub>\<C>)
+      with C X have "chained_closure \<Delta> (Lam\<^sub>v p\<^sub>\<Delta> p\<^sub>\<C>)" by (metis hlookup_all)
+      with S A Lam\<^sub>v show ?thesis by auto
+    qed simp_all
+  qed
+  thus "hmap (unchain_closure \<Delta>') h = hmap (unchain_closure \<Delta>) h" by (metis hmap_eq)
+qed
+
+lemma halloc_unchain_stack [elim]: "chained_stack \<Delta> s \<Longrightarrow> halloc \<Delta> v = (\<Delta>', p) \<Longrightarrow> 
+    unchain_stack \<Delta>' s = unchain_stack \<Delta> s"
+  by (induction s) auto
+
+lemma unfold_unstack_list [simp]: "chain_structured h \<Delta> \<Longrightarrow> chained_heap_pointer \<Delta> p \<Longrightarrow> 
+  halloc \<Delta> (v, p) = (\<Delta>', p') \<Longrightarrow> unchain_env \<Delta>' (Suc p') = v # unchain_env \<Delta> p"
+proof -
+  assume A: "chain_structured h \<Delta>"
+  assume B: "chained_heap_pointer \<Delta> p"
+  assume C: "halloc \<Delta> (v, p) = (\<Delta>', p')"
+  moreover with A B have "unchain_env \<Delta>' p = unchain_env \<Delta> p" by simp
   moreover have "p \<le> p'" 
   proof (cases p)
     case (Suc pp)
@@ -106,384 +168,285 @@ proof -
   ultimately show ?thesis by simp
 qed
 
-lemma [simp]: "chain_structured h env \<Longrightarrow> chained_stack_pointer env p \<Longrightarrow>
-  lookup (unstack_list env p) x = chain_lookup env p x"
-proof (induction env p x rule: chain_lookup.induct)
-  case (3 env p x)
-  obtain v p' where V: "hlookup env p = (v, p')" by (cases "hlookup env p")
-  from 3 have "hcontains env p" by auto
-  with 3 V have P: "p' \<le> p" using hlookup_all by fast
-  with 3 V have "chained_stack_pointer env p'" by auto
-  with 3(1, 2) V P show ?case by fastforce
-qed (simp_all split: prod.splits)
+text \<open>Completeness follows:\<close>
 
-lemma [simp]: "halloc h (Const\<^sub>v k) = (h', p) \<Longrightarrow> 
-  halloc (unchain_heap h env) (Const\<^sub>h k) = (unchain_heap h' env, p)"
-proof -
-  assume "halloc h (Const\<^sub>v k) = (h', p)"
-  hence "halloc (hmap (unchain_closure env) h) (unchain_closure env (Const\<^sub>v k)) = 
-    (hmap (unchain_closure env) h', p)" by (metis halloc_map)
-  thus ?thesis by (simp add: unchain_heap_def)
-qed
+theorem complete\<^sub>v [simp]: "\<C> \<tturnstile> \<Sigma>\<^sub>v \<leadsto>\<^sub>v \<Sigma>\<^sub>v' \<Longrightarrow> chained_state \<Sigma>\<^sub>v \<Longrightarrow> 
+  \<C> \<tturnstile> unchain_state \<Sigma>\<^sub>v \<leadsto>\<^sub>h unchain_state \<Sigma>\<^sub>v'"
+proof (induction \<Sigma>\<^sub>v \<Sigma>\<^sub>v' rule: eval\<^sub>v.induct)
+  case (ev\<^sub>v_apply \<C> p\<^sub>\<C> h\<^sub>v v\<^sub>2 p\<^sub>\<Delta>' p\<^sub>\<C>' \<Delta>\<^sub>v v\<^sub>1 \<Delta>\<^sub>v' p\<^sub>\<Delta>'' \<V> p\<^sub>\<Delta> s\<^sub>v)
+  from ev\<^sub>v_apply have "chained_closures \<Delta>\<^sub>v h\<^sub>v \<and> hcontains h\<^sub>v v\<^sub>2" by simp
+  with ev\<^sub>v_apply have "chained_closure \<Delta>\<^sub>v (Lam\<^sub>v p\<^sub>\<Delta>' p\<^sub>\<C>')" by (metis hlookup_all)
+  with ev\<^sub>v_apply have "chain_structured h\<^sub>v \<Delta>\<^sub>v \<and> chained_heap_pointer \<Delta>\<^sub>v p\<^sub>\<Delta>' \<and> 
+    halloc \<Delta>\<^sub>v (v\<^sub>1, p\<^sub>\<Delta>') = (\<Delta>\<^sub>v', p\<^sub>\<Delta>'')" by auto
+  hence X: "unchain_env \<Delta>\<^sub>v' (Suc p\<^sub>\<Delta>'') = v\<^sub>1 # unchain_env \<Delta>\<^sub>v p\<^sub>\<Delta>'" by (metis unfold_unstack_list)
+  from ev\<^sub>v_apply have A: "unchain_heap h\<^sub>v \<Delta>\<^sub>v' = unchain_heap h\<^sub>v \<Delta>\<^sub>v" by auto
+  from ev\<^sub>v_apply have B: "unchain_env \<Delta>\<^sub>v' p\<^sub>\<Delta> = unchain_env \<Delta>\<^sub>v p\<^sub>\<Delta>" by auto
+  from ev\<^sub>v_apply have "chained_stack \<Delta>\<^sub>v s\<^sub>v" by simp
+  with ev\<^sub>v_apply have C: "unchain_stack \<Delta>\<^sub>v' s\<^sub>v = unchain_stack \<Delta>\<^sub>v s\<^sub>v" by fastforce
+  with ev\<^sub>v_apply X A B have "\<C> \<tturnstile> S\<^sub>h (unchain_heap h\<^sub>v \<Delta>\<^sub>v) (v\<^sub>1 # v\<^sub>2 # \<V>) 
+    ((unchain_env \<Delta>\<^sub>v p\<^sub>\<Delta>, Suc p\<^sub>\<C>) # unchain_stack \<Delta>\<^sub>v s\<^sub>v) \<leadsto>\<^sub>h
+      S\<^sub>h (unchain_heap h\<^sub>v \<Delta>\<^sub>v') \<V> 
+        ((unchain_env \<Delta>\<^sub>v' (Suc p\<^sub>\<Delta>''), p\<^sub>\<C>') # (unchain_env \<Delta>\<^sub>v' p\<^sub>\<Delta>, p\<^sub>\<C>) # unchain_stack \<Delta>\<^sub>v' s\<^sub>v)" 
+    by (simp add: C)
+  thus ?case by simp
+next
+  case (ev\<^sub>v_jump \<C> p\<^sub>\<C> h\<^sub>v v\<^sub>2 p\<^sub>\<Delta>' p\<^sub>\<C>' \<Delta>\<^sub>v v\<^sub>1 \<Delta>\<^sub>v' p\<^sub>\<Delta>'' \<V> p\<^sub>\<Delta> s\<^sub>v)
+  from ev\<^sub>v_jump have "chained_closures \<Delta>\<^sub>v h\<^sub>v \<and> hcontains h\<^sub>v v\<^sub>2" by simp
+  with ev\<^sub>v_jump have "chained_closure \<Delta>\<^sub>v (Lam\<^sub>v p\<^sub>\<Delta>' p\<^sub>\<C>')" by (metis hlookup_all)
+  with ev\<^sub>v_jump have "chain_structured h\<^sub>v \<Delta>\<^sub>v \<and> chained_heap_pointer \<Delta>\<^sub>v p\<^sub>\<Delta>' \<and> 
+    halloc \<Delta>\<^sub>v (v\<^sub>1, p\<^sub>\<Delta>') = (\<Delta>\<^sub>v', p\<^sub>\<Delta>'')" by auto
+  hence X: "unchain_env \<Delta>\<^sub>v' (Suc p\<^sub>\<Delta>'') = v\<^sub>1 # unchain_env \<Delta>\<^sub>v p\<^sub>\<Delta>'" by (metis unfold_unstack_list)
+  from ev\<^sub>v_jump have A: "unchain_heap h\<^sub>v \<Delta>\<^sub>v' = unchain_heap h\<^sub>v \<Delta>\<^sub>v" by auto
+  from ev\<^sub>v_jump have "chained_stack \<Delta>\<^sub>v s\<^sub>v" by simp
+  with ev\<^sub>v_jump have B: "unchain_stack \<Delta>\<^sub>v' s\<^sub>v = unchain_stack \<Delta>\<^sub>v s\<^sub>v" by fastforce 
+  with ev\<^sub>v_jump X A have "\<C> \<tturnstile> S\<^sub>h (unchain_heap h\<^sub>v \<Delta>\<^sub>v) (v\<^sub>1 # v\<^sub>2 # \<V>) 
+    ((unchain_env \<Delta>\<^sub>v p\<^sub>\<Delta>, Suc p\<^sub>\<C>) # unchain_stack \<Delta>\<^sub>v s\<^sub>v) \<leadsto>\<^sub>h
+      S\<^sub>h (unchain_heap h\<^sub>v \<Delta>\<^sub>v') \<V> 
+        ((unchain_env \<Delta>\<^sub>v' (Suc p\<^sub>\<Delta>''), p\<^sub>\<C>') # unchain_stack \<Delta>\<^sub>v' s\<^sub>v)" by (simp add: B)
+  thus ?case by simp
+qed auto
 
-lemma [simp]: "halloc h (Lam\<^sub>v p pc) = (h', v) \<Longrightarrow> 
-  halloc (unchain_heap h env) (Lam\<^sub>h (unstack_list env p) pc) = (unchain_heap h' env, v)"
-proof -
-  assume "halloc h (Lam\<^sub>v p pc) = (h', v)"
-  hence "halloc (hmap (unchain_closure env) h) (unchain_closure env (Lam\<^sub>v p pc)) = 
-    (hmap (unchain_closure env) h', v)" by (metis halloc_map)
-  thus ?thesis by (simp add: unchain_heap_def)
-qed
+text \<open>There are few reconstruction lemmas this stage, but correctness is still somewhat involved.\<close>
 
-lemma [simp]: "hlookup h x = Const\<^sub>v k \<Longrightarrow> hcontains h x \<Longrightarrow> 
-    hlookup (unchain_heap h env) x = Const\<^sub>h k"
-  by (simp add: unchain_heap_def)
+lemma unchain_state_reverse [dest]: "S\<^sub>h h\<^sub>h \<V> s\<^sub>h = unchain_state \<Sigma>\<^sub>v \<Longrightarrow> 
+    \<exists>h\<^sub>v \<Delta>\<^sub>v s\<^sub>v. \<Sigma>\<^sub>v = S\<^sub>v h\<^sub>v \<Delta>\<^sub>v \<V> s\<^sub>v \<and> h\<^sub>h = unchain_heap h\<^sub>v \<Delta>\<^sub>v \<and> s\<^sub>h = unchain_stack \<Delta>\<^sub>v s\<^sub>v"
+  by (induction \<Sigma>\<^sub>v) simp_all
 
-lemma [simp]: "hlookup h x = Lam\<^sub>v p pc \<Longrightarrow> hcontains h x \<Longrightarrow> 
-    hlookup (unchain_heap h env) x = Lam\<^sub>h (unstack_list env p) pc"
-  by (simp add: unchain_heap_def)
-
-lemma unchain_state_reverse [dest]: "S\<^sub>h h vs sfs = unchain_state \<Sigma> \<Longrightarrow> 
-  \<exists>h\<^sub>c\<^sub>e env sfs\<^sub>c\<^sub>e. \<Sigma> = S\<^sub>v h\<^sub>c\<^sub>e env vs sfs\<^sub>c\<^sub>e \<and> h = unchain_heap h\<^sub>c\<^sub>e env \<and> 
-    sfs = unchain_stack env sfs\<^sub>c\<^sub>e"
-  by (induction \<Sigma>) simp_all
-
-lemma [dest]: "Lam\<^sub>h env\<^sub>h pc = unchain_closure env\<^sub>c\<^sub>e x \<Longrightarrow> 
-    \<exists>p. x = Lam\<^sub>v p pc \<and> env\<^sub>h = unstack_list env\<^sub>c\<^sub>e p"
+lemma unchain_lam_reverse [dest]: "Lam\<^sub>h \<Delta>\<^sub>h p\<^sub>C = unchain_closure \<Delta>\<^sub>v x \<Longrightarrow> 
+    \<exists>p\<^sub>\<Delta>. x = Lam\<^sub>v p\<^sub>\<Delta> p\<^sub>C \<and> \<Delta>\<^sub>h = unchain_env \<Delta>\<^sub>v p\<^sub>\<Delta>"
   by (induction x) simp_all
 
-lemma [elim]: "hcontains env p \<Longrightarrow> halloc env v = (env', q) \<Longrightarrow> 
-    unstack_list env' p = unstack_list env p"
-proof (induction env p rule: unstack_list.induct)
-  case (2 env p)
-  obtain vv p' where V: "hlookup env p = (vv, p')" by (cases "hlookup env p")
-  from 2(2) have "hcontains env p" by fast
-  with 2(3) V have V': "hlookup env' p = (vv, p')" by simp
-  from 2(2) V have "p' \<le> p \<Longrightarrow> hcontains env p'" by auto
-  with 2 V have "p' \<le> p \<Longrightarrow> unstack_list env' p' = unstack_list env p'" by metis
-  with V V' show ?case by simp
-qed simp_all
-
-lemma [elim]: "chain_structured h env \<Longrightarrow> chained_closures env h \<Longrightarrow> halloc env v = (env', p) \<Longrightarrow> 
-  unchain_heap h env' = unchain_heap h env"
-proof (unfold unchain_heap_def)
-  assume S: "chain_structured h env" and C: "chained_closures env h" 
-    and A: "halloc env v = (env', p)"
-  have "\<And>x. hcontains h x \<Longrightarrow> unchain_closure env' (hlookup h x) = 
-    unchain_closure env (hlookup h x)" 
-  proof -
-    fix x
-    assume X: "hcontains h x"
-    show "unchain_closure env' (hlookup h x) = unchain_closure env (hlookup h x)" 
-    proof (cases "hlookup h x")
-      case (Lam\<^sub>v pp pc)
-      with C X have "chained_closure env (Lam\<^sub>v pp pc)" by (metis hlookup_all)
-      with S A Lam\<^sub>v show ?thesis by auto
-    qed simp_all
-  qed
-  thus "hmap (unchain_closure env') h = hmap (unchain_closure env) h" by (metis hmap_eq)
-qed
-
-lemma [elim]: "chained_stack_pointer env a \<Longrightarrow> halloc env v = (env', p) \<Longrightarrow> 
-  unstack_list env' a = unstack_list env a"
-proof (induction a)
-  case (Suc p)
-  moreover obtain v' p' where "hlookup env p = (v', p')" by (cases "hlookup env p")
-  moreover from Suc have "p' \<le> p \<Longrightarrow> hcontains env p'" by auto
-  ultimately show ?case by auto
-qed simp_all
-
-lemma [elim]: "chained_frame env a \<Longrightarrow> halloc env v = (env', p) \<Longrightarrow> 
-    unchain_frame env' a = unchain_frame env a"
-  by (induction a) auto
-
-lemma [elim]: "chained_stack env sfs \<Longrightarrow> halloc env v = (env', p) \<Longrightarrow> 
-    unchain_stack env' sfs = unchain_stack env sfs"
-  by (induction sfs) (auto simp add: unchain_stack_def)
-
-theorem completece [simp]: "cd \<tturnstile> unchain_state \<Sigma>\<^sub>c\<^sub>e \<leadsto>\<^sub>h \<Sigma>\<^sub>h \<Longrightarrow> chained_state \<Sigma>\<^sub>c\<^sub>e \<Longrightarrow>
-  \<exists>\<Sigma>\<^sub>c\<^sub>e'. (cd \<tturnstile> \<Sigma>\<^sub>c\<^sub>e \<leadsto>\<^sub>v \<Sigma>\<^sub>c\<^sub>e') \<and> \<Sigma>\<^sub>h = unchain_state \<Sigma>\<^sub>c\<^sub>e'"
-proof (induction "unchain_state \<Sigma>\<^sub>c\<^sub>e" \<Sigma>\<^sub>h arbitrary: \<Sigma>\<^sub>c\<^sub>e rule: eval\<^sub>h.induct)
-  case (ev\<^sub>h_lookup cd pc x env v h vs sfs)
-  then obtain h\<^sub>c\<^sub>e env\<^sub>c\<^sub>e sfs\<^sub>c\<^sub>e' where S: "\<Sigma>\<^sub>c\<^sub>e = S\<^sub>v h\<^sub>c\<^sub>e env\<^sub>c\<^sub>e vs sfs\<^sub>c\<^sub>e' \<and> h = unchain_heap h\<^sub>c\<^sub>e env\<^sub>c\<^sub>e \<and> 
-    (env, Suc pc) # sfs = unchain_stack env\<^sub>c\<^sub>e sfs\<^sub>c\<^sub>e'" by fastforce
-  then obtain sf\<^sub>c\<^sub>e sfs\<^sub>c\<^sub>e where SF: "sfs\<^sub>c\<^sub>e' = sf\<^sub>c\<^sub>e # sfs\<^sub>c\<^sub>e \<and> (env, Suc pc) = unchain_frame env\<^sub>c\<^sub>e sf\<^sub>c\<^sub>e \<and> 
-    sfs = unchain_stack env\<^sub>c\<^sub>e sfs\<^sub>c\<^sub>e" by (auto simp add: unchain_stack_def)
-  then obtain p where P: "sf\<^sub>c\<^sub>e = (p, Suc pc) \<and> env = unstack_list env\<^sub>c\<^sub>e p" by (cases sf\<^sub>c\<^sub>e) simp_all
-  with ev\<^sub>h_lookup S SF have C: "chain_structured h\<^sub>c\<^sub>e env\<^sub>c\<^sub>e" by simp
-  with ev\<^sub>h_lookup S SF P have X: "S\<^sub>h h (v # vs) ((env, pc) # sfs) = 
-    unchain_state (S\<^sub>v h\<^sub>c\<^sub>e env\<^sub>c\<^sub>e (v # vs) ((p, pc) # sfs\<^sub>c\<^sub>e))" by (simp add: unchain_stack_def)
-  from ev\<^sub>h_lookup S SF P have "chained_frame env\<^sub>c\<^sub>e (p, Suc pc)" by simp
-  with C have "lookup (unstack_list env\<^sub>c\<^sub>e p) x = chain_lookup env\<^sub>c\<^sub>e p x" by simp
-  with ev\<^sub>h_lookup P C have "cd \<tturnstile> S\<^sub>v h\<^sub>c\<^sub>e env\<^sub>c\<^sub>e vs ((p, Suc pc) # sfs\<^sub>c\<^sub>e) \<leadsto>\<^sub>v 
-    S\<^sub>v h\<^sub>c\<^sub>e env\<^sub>c\<^sub>e (v # vs) ((p, pc) # sfs\<^sub>c\<^sub>e)" by simp
-  with S SF P X show ?case by blast
-next
-  case (ev\<^sub>h_pushcon cd pc k h h' v vs env sfs)
-  then obtain h\<^sub>c\<^sub>e env\<^sub>c\<^sub>e sfs\<^sub>c\<^sub>e' where S: "\<Sigma>\<^sub>c\<^sub>e = S\<^sub>v h\<^sub>c\<^sub>e env\<^sub>c\<^sub>e vs sfs\<^sub>c\<^sub>e' \<and> h = unchain_heap h\<^sub>c\<^sub>e env\<^sub>c\<^sub>e \<and> 
-    (env, Suc pc) # sfs = unchain_stack env\<^sub>c\<^sub>e sfs\<^sub>c\<^sub>e'" by fastforce
-  then obtain sf\<^sub>c\<^sub>e sfs\<^sub>c\<^sub>e where SF: "sfs\<^sub>c\<^sub>e' = sf\<^sub>c\<^sub>e # sfs\<^sub>c\<^sub>e \<and> (env, Suc pc) = unchain_frame env\<^sub>c\<^sub>e sf\<^sub>c\<^sub>e \<and> 
-    sfs = unchain_stack env\<^sub>c\<^sub>e sfs\<^sub>c\<^sub>e" by (auto simp add: unchain_stack_def)
-  then obtain p where P: "sf\<^sub>c\<^sub>e = (p, Suc pc) \<and> env = unstack_list env\<^sub>c\<^sub>e p" by (cases sf\<^sub>c\<^sub>e) simp_all
-  from ev\<^sub>h_pushcon S have "halloc (hmap (unchain_closure env\<^sub>c\<^sub>e) h\<^sub>c\<^sub>e) 
-    (unchain_closure env\<^sub>c\<^sub>e (Const\<^sub>v k)) = (h', v)" by (simp add: unchain_heap_def)
-  then obtain h\<^sub>c\<^sub>e' where H: "halloc h\<^sub>c\<^sub>e (Const\<^sub>v k) = (h\<^sub>c\<^sub>e', v) \<and> 
-    h' = hmap (unchain_closure env\<^sub>c\<^sub>e) h\<^sub>c\<^sub>e'" by (metis halloc_map_inv)
-  hence "h' = unchain_heap h\<^sub>c\<^sub>e' env\<^sub>c\<^sub>e" by (simp add: unchain_heap_def)
-  with SF P have X: "S\<^sub>h h' (v # vs) ((env, pc) # sfs) = 
-    unchain_state (S\<^sub>v h\<^sub>c\<^sub>e' env\<^sub>c\<^sub>e (v # vs) ((p, pc) # sfs\<^sub>c\<^sub>e))" by (simp add: unchain_stack_def)
-  from ev\<^sub>h_pushcon H have "cd \<tturnstile> S\<^sub>v h\<^sub>c\<^sub>e env\<^sub>c\<^sub>e vs ((p, Suc pc) # sfs\<^sub>c\<^sub>e) \<leadsto>\<^sub>v 
-    S\<^sub>v h\<^sub>c\<^sub>e' env\<^sub>c\<^sub>e (v # vs) ((p, pc) # sfs\<^sub>c\<^sub>e)" by simp
-  with S SF P X show ?case by blast
-next
-  case (ev\<^sub>h_pushlam cd pc pc' h env h' v vs sfs)
-  then obtain h\<^sub>c\<^sub>e env\<^sub>c\<^sub>e sfs\<^sub>c\<^sub>e' where S: "\<Sigma>\<^sub>c\<^sub>e = S\<^sub>v h\<^sub>c\<^sub>e env\<^sub>c\<^sub>e vs sfs\<^sub>c\<^sub>e' \<and> h = unchain_heap h\<^sub>c\<^sub>e env\<^sub>c\<^sub>e \<and> 
-    (env, Suc pc) # sfs = unchain_stack env\<^sub>c\<^sub>e sfs\<^sub>c\<^sub>e'" by fastforce
-  then obtain sf\<^sub>c\<^sub>e sfs\<^sub>c\<^sub>e where SF: "sfs\<^sub>c\<^sub>e' = sf\<^sub>c\<^sub>e # sfs\<^sub>c\<^sub>e \<and> (env, Suc pc) = unchain_frame env\<^sub>c\<^sub>e sf\<^sub>c\<^sub>e \<and> 
-    sfs = unchain_stack env\<^sub>c\<^sub>e sfs\<^sub>c\<^sub>e" by (auto simp add: unchain_stack_def)
-  then obtain p where P: "sf\<^sub>c\<^sub>e = (p, Suc pc) \<and> env = unstack_list env\<^sub>c\<^sub>e p" by (cases sf\<^sub>c\<^sub>e) simp_all
-  with ev\<^sub>h_pushlam S have "halloc (hmap (unchain_closure env\<^sub>c\<^sub>e) h\<^sub>c\<^sub>e) 
-    (unchain_closure env\<^sub>c\<^sub>e (Lam\<^sub>v p pc')) = (h', v)" by (simp add: unchain_heap_def)
-  then obtain h\<^sub>c\<^sub>e' where H: "halloc h\<^sub>c\<^sub>e (Lam\<^sub>v p pc') = (h\<^sub>c\<^sub>e', v) \<and> 
-    h' = hmap (unchain_closure env\<^sub>c\<^sub>e) h\<^sub>c\<^sub>e'" by (metis halloc_map_inv)
-  hence "h' = unchain_heap h\<^sub>c\<^sub>e' env\<^sub>c\<^sub>e" by (simp add: unchain_heap_def)
-  with SF P have X: "S\<^sub>h h' (v # vs) ((env, pc) # sfs) = 
-    unchain_state (S\<^sub>v h\<^sub>c\<^sub>e' env\<^sub>c\<^sub>e (v # vs) ((p, pc) # sfs\<^sub>c\<^sub>e))" by (simp add: unchain_stack_def)
-  from ev\<^sub>h_pushlam H have "cd \<tturnstile> S\<^sub>v h\<^sub>c\<^sub>e env\<^sub>c\<^sub>e vs ((p, Suc pc) # sfs\<^sub>c\<^sub>e) \<leadsto>\<^sub>v 
-    S\<^sub>v h\<^sub>c\<^sub>e' env\<^sub>c\<^sub>e (v # vs) ((p, pc) # sfs\<^sub>c\<^sub>e)" by simp
-  with S SF P X show ?case by blast
-next
-  case (ev\<^sub>h_apply cd pc h v2 env' pc' v1 vs env sfs)
-  then obtain h\<^sub>c\<^sub>e env\<^sub>c\<^sub>e sfs\<^sub>c\<^sub>e' where S: "\<Sigma>\<^sub>c\<^sub>e = S\<^sub>v h\<^sub>c\<^sub>e env\<^sub>c\<^sub>e (v1 # v2 # vs) sfs\<^sub>c\<^sub>e' \<and> 
-    h = unchain_heap h\<^sub>c\<^sub>e env\<^sub>c\<^sub>e \<and> (env, Suc pc) # sfs = unchain_stack env\<^sub>c\<^sub>e sfs\<^sub>c\<^sub>e'" by fastforce
-  then obtain sf\<^sub>c\<^sub>e sfs\<^sub>c\<^sub>e where SF: "sfs\<^sub>c\<^sub>e' = sf\<^sub>c\<^sub>e # sfs\<^sub>c\<^sub>e \<and> (env, Suc pc) = unchain_frame env\<^sub>c\<^sub>e sf\<^sub>c\<^sub>e \<and> 
-    sfs = unchain_stack env\<^sub>c\<^sub>e sfs\<^sub>c\<^sub>e" by (auto simp add: unchain_stack_def)
-  then obtain p where P: "sf\<^sub>c\<^sub>e = (p, Suc pc) \<and> env = unstack_list env\<^sub>c\<^sub>e p" by (cases sf\<^sub>c\<^sub>e) simp_all
-  from ev\<^sub>h_apply S have "Lam\<^sub>h env' pc' = unchain_closure env\<^sub>c\<^sub>e (hlookup h\<^sub>c\<^sub>e v2)" 
-    by (simp add: unchain_heap_def)
-  then obtain p' where P': "hlookup h\<^sub>c\<^sub>e v2 = Lam\<^sub>v p' pc' \<and> env' = unstack_list env\<^sub>c\<^sub>e p'" by blast
-  obtain env\<^sub>c\<^sub>e' p'' where H: "halloc env\<^sub>c\<^sub>e (v1, p') = (env\<^sub>c\<^sub>e', p'')" 
-    by (cases "halloc env\<^sub>c\<^sub>e (v1, p')") simp_all
-  from ev\<^sub>h_apply S SF P have C: "chain_structured h\<^sub>c\<^sub>e env\<^sub>c\<^sub>e \<and> chained_closures env\<^sub>c\<^sub>e h\<^sub>c\<^sub>e \<and>
-    hcontains h\<^sub>c\<^sub>e v1 \<and> hcontains h\<^sub>c\<^sub>e v2 \<and> chained_vals h\<^sub>c\<^sub>e vs \<and> chained_frame env\<^sub>c\<^sub>e (p, Suc pc) \<and> 
-      chained_stack env\<^sub>c\<^sub>e sfs\<^sub>c\<^sub>e" by simp
-  with H have Y: "unchain_heap h\<^sub>c\<^sub>e env\<^sub>c\<^sub>e' = unchain_heap h\<^sub>c\<^sub>e env\<^sub>c\<^sub>e" by fast
-  from H C have "unstack_list env\<^sub>c\<^sub>e' p = unstack_list env\<^sub>c\<^sub>e p" by fastforce
-  with P have W: "env = unstack_list env\<^sub>c\<^sub>e' p" by metis
-  from P' C have "chained_closure env\<^sub>c\<^sub>e (Lam\<^sub>v p' pc')" by (metis hlookup_all)
-  hence "chained_stack_pointer env\<^sub>c\<^sub>e p'" by auto
-  with H C have "unstack_list env\<^sub>c\<^sub>e' (Suc p'') = v1 # unstack_list env\<^sub>c\<^sub>e p'" 
-    by (metis unfold_unstack_list)
-  with H P' have Z: "v1 # env' = unstack_list env\<^sub>c\<^sub>e' (Suc p'')" by simp
-  from H C have "unchain_stack env\<^sub>c\<^sub>e' sfs\<^sub>c\<^sub>e = unchain_stack env\<^sub>c\<^sub>e sfs\<^sub>c\<^sub>e" by fast
-  with SF have "sfs = unchain_stack env\<^sub>c\<^sub>e' sfs\<^sub>c\<^sub>e" by simp
-  with S Y Z W have X: "S\<^sub>h h vs ((v1 # env', pc') # (env, pc) # sfs) = 
-    unchain_state (S\<^sub>v h\<^sub>c\<^sub>e env\<^sub>c\<^sub>e' vs ((Suc p'', pc') # (p, pc) # sfs\<^sub>c\<^sub>e))" 
-      by (simp add: unchain_stack_def)
-  from ev\<^sub>h_apply P' H have "cd \<tturnstile> S\<^sub>v h\<^sub>c\<^sub>e env\<^sub>c\<^sub>e (v1 # v2 # vs) ((p, Suc pc) # sfs\<^sub>c\<^sub>e) \<leadsto>\<^sub>v 
-      S\<^sub>v h\<^sub>c\<^sub>e env\<^sub>c\<^sub>e' vs ((Suc p'', pc') # (p, pc) # sfs\<^sub>c\<^sub>e)" by simp
-  with S SF P X show ?case by blast
-next
-  case (ev\<^sub>h_return cd pc h vs env sfs)
-  then obtain h\<^sub>c\<^sub>e env\<^sub>c\<^sub>e sfs\<^sub>c\<^sub>e' where S: "\<Sigma>\<^sub>c\<^sub>e = S\<^sub>v h\<^sub>c\<^sub>e env\<^sub>c\<^sub>e vs sfs\<^sub>c\<^sub>e' \<and> h = unchain_heap h\<^sub>c\<^sub>e env\<^sub>c\<^sub>e \<and> 
-    (env, Suc pc) # sfs = unchain_stack env\<^sub>c\<^sub>e sfs\<^sub>c\<^sub>e'" by fastforce
-  then obtain sf\<^sub>c\<^sub>e sfs\<^sub>c\<^sub>e where SF: "sfs\<^sub>c\<^sub>e' = sf\<^sub>c\<^sub>e # sfs\<^sub>c\<^sub>e \<and> (env, Suc pc) = unchain_frame env\<^sub>c\<^sub>e sf\<^sub>c\<^sub>e \<and> 
-    sfs = unchain_stack env\<^sub>c\<^sub>e sfs\<^sub>c\<^sub>e" by (auto simp add: unchain_stack_def)
-  then obtain p where P: "sf\<^sub>c\<^sub>e = (p, Suc pc) \<and> env = unstack_list env\<^sub>c\<^sub>e p" by (cases sf\<^sub>c\<^sub>e) simp_all
-  from S SF have X: "S\<^sub>h h vs sfs = unchain_state (S\<^sub>v h\<^sub>c\<^sub>e env\<^sub>c\<^sub>e vs sfs\<^sub>c\<^sub>e)" by simp
-  from ev\<^sub>h_return have "cd \<tturnstile> S\<^sub>v h\<^sub>c\<^sub>e env\<^sub>c\<^sub>e vs ((p, Suc pc) # sfs\<^sub>c\<^sub>e) \<leadsto>\<^sub>v S\<^sub>v h\<^sub>c\<^sub>e env\<^sub>c\<^sub>e vs sfs\<^sub>c\<^sub>e" by simp
-  with S SF P X show ?case by blast
-next
-  case (ev\<^sub>h_jump cd pc h v2 env' pc' v1 vs env sfs)
-  then obtain h\<^sub>c\<^sub>e env\<^sub>c\<^sub>e sfs\<^sub>c\<^sub>e' where S: "\<Sigma>\<^sub>c\<^sub>e = S\<^sub>v h\<^sub>c\<^sub>e env\<^sub>c\<^sub>e (v1 # v2 # vs) sfs\<^sub>c\<^sub>e' \<and> 
-    h = unchain_heap h\<^sub>c\<^sub>e env\<^sub>c\<^sub>e \<and> (env, Suc pc) # sfs = unchain_stack env\<^sub>c\<^sub>e sfs\<^sub>c\<^sub>e'" by fastforce
-  then obtain sf\<^sub>c\<^sub>e sfs\<^sub>c\<^sub>e where SF: "sfs\<^sub>c\<^sub>e' = sf\<^sub>c\<^sub>e # sfs\<^sub>c\<^sub>e \<and> (env, Suc pc) = unchain_frame env\<^sub>c\<^sub>e sf\<^sub>c\<^sub>e \<and> 
-    sfs = unchain_stack env\<^sub>c\<^sub>e sfs\<^sub>c\<^sub>e" by (auto simp add: unchain_stack_def)
-  then obtain p where P: "sf\<^sub>c\<^sub>e = (p, Suc pc) \<and> env = unstack_list env\<^sub>c\<^sub>e p" by (cases sf\<^sub>c\<^sub>e) simp_all
-  from ev\<^sub>h_jump S have "Lam\<^sub>h env' pc' = unchain_closure env\<^sub>c\<^sub>e (hlookup h\<^sub>c\<^sub>e v2)" 
-    by (simp add: unchain_heap_def)
-  then obtain p' where P': "hlookup h\<^sub>c\<^sub>e v2 = Lam\<^sub>v p' pc' \<and> env' = unstack_list env\<^sub>c\<^sub>e p'" by blast
-  obtain env\<^sub>c\<^sub>e' p'' where H: "halloc env\<^sub>c\<^sub>e (v1, p') = (env\<^sub>c\<^sub>e', p'')" 
-    by (cases "halloc env\<^sub>c\<^sub>e (v1, p')") simp_all
-  from ev\<^sub>h_jump S SF P have C: "chain_structured h\<^sub>c\<^sub>e env\<^sub>c\<^sub>e \<and> chained_closures env\<^sub>c\<^sub>e h\<^sub>c\<^sub>e \<and>
-    hcontains h\<^sub>c\<^sub>e v1 \<and> hcontains h\<^sub>c\<^sub>e v2 \<and> chained_vals h\<^sub>c\<^sub>e vs \<and> chained_stack_pointer env\<^sub>c\<^sub>e p \<and> 
-      chained_stack env\<^sub>c\<^sub>e sfs\<^sub>c\<^sub>e" by simp
-  with H have Y: "unchain_heap h\<^sub>c\<^sub>e env\<^sub>c\<^sub>e' = unchain_heap h\<^sub>c\<^sub>e env\<^sub>c\<^sub>e" by fast
-  from P' C have "chained_closure env\<^sub>c\<^sub>e (Lam\<^sub>v p' pc')" by (metis hlookup_all)
-  hence "chained_stack_pointer env\<^sub>c\<^sub>e p'" by simp
-  with H C have "unstack_list env\<^sub>c\<^sub>e' (Suc p'') = v1 # unstack_list env\<^sub>c\<^sub>e p'" 
-    by (metis unfold_unstack_list)
-  with H P' have Z: "v1 # env' = unstack_list env\<^sub>c\<^sub>e' (Suc p'')" by simp
-  from H C have "unchain_stack env\<^sub>c\<^sub>e' sfs\<^sub>c\<^sub>e = unchain_stack env\<^sub>c\<^sub>e sfs\<^sub>c\<^sub>e" by fast
-  with SF have "sfs = unchain_stack env\<^sub>c\<^sub>e' sfs\<^sub>c\<^sub>e" by simp
-  with S Y Z have X: "S\<^sub>h h vs ((v1 # env', pc') # sfs) = 
-    unchain_state (S\<^sub>v h\<^sub>c\<^sub>e env\<^sub>c\<^sub>e' vs ((Suc p'', pc') # sfs\<^sub>c\<^sub>e))" by (simp add: unchain_stack_def)
-  from ev\<^sub>h_jump P' H have "cd \<tturnstile> S\<^sub>v h\<^sub>c\<^sub>e env\<^sub>c\<^sub>e (v1 # v2 # vs) ((p, Suc pc) # sfs\<^sub>c\<^sub>e) \<leadsto>\<^sub>v 
-      S\<^sub>v h\<^sub>c\<^sub>e env\<^sub>c\<^sub>e' vs ((Suc p'', pc') # sfs\<^sub>c\<^sub>e)" by simp
-  with S SF P X show ?case by blast
-qed
-
-theorem correctce [simp]: "cd \<tturnstile> \<Sigma>\<^sub>c\<^sub>e \<leadsto>\<^sub>v \<Sigma>\<^sub>c\<^sub>e' \<Longrightarrow> chained_state \<Sigma>\<^sub>c\<^sub>e \<Longrightarrow> 
-  cd \<tturnstile> unchain_state \<Sigma>\<^sub>c\<^sub>e \<leadsto>\<^sub>h unchain_state \<Sigma>\<^sub>c\<^sub>e'"
-proof (induction \<Sigma>\<^sub>c\<^sub>e \<Sigma>\<^sub>c\<^sub>e' rule: eval\<^sub>v.induct)
-  case (ev\<^sub>v_lookup cd pc x env p v h vs sfs)
-  moreover hence "lookup (unstack_list env p) x = chain_lookup env p x" by auto
-  ultimately show ?case by (simp add: unchain_stack_def)
-next
-  case (ev\<^sub>v_apply cd pc h v2 p' pc' env v1 env' p'' vs p sfs)
-  from ev\<^sub>v_apply have "chained_closures env h \<and> hcontains h v2" by simp
-  with ev\<^sub>v_apply have "chained_closure env (Lam\<^sub>v p' pc')" by (metis hlookup_all)
-  with ev\<^sub>v_apply have "chain_structured h env \<and> chained_stack_pointer env p' \<and> 
-    halloc env (v1, p') = (env', p'')" by auto
-  hence X: "unstack_list env' (Suc p'') = v1 # unstack_list env p'" by (metis unfold_unstack_list)
-  from ev\<^sub>v_apply have A: "unchain_heap h env' = unchain_heap h env" by auto
-  from ev\<^sub>v_apply have B: "unstack_list env' p = unstack_list env p" by auto
-  from ev\<^sub>v_apply have "unchain_stack env' sfs = unchain_stack env sfs" by auto 
-  with ev\<^sub>v_apply X A B have "cd \<tturnstile> S\<^sub>h (unchain_heap h env) (v1 # v2 # vs) 
-    ((unstack_list env p, Suc pc) # unchain_stack env sfs) \<leadsto>\<^sub>h
-      S\<^sub>h (unchain_heap h env') vs 
-        ((unstack_list env' (Suc p''), pc') # (unstack_list env' p, pc) # unchain_stack env' sfs)" 
+theorem correct\<^sub>v [simp]: "\<C> \<tturnstile> unchain_state \<Sigma>\<^sub>v \<leadsto>\<^sub>h \<Sigma>\<^sub>h \<Longrightarrow> chained_state \<Sigma>\<^sub>v \<Longrightarrow>
+  \<exists>\<Sigma>\<^sub>v'. (\<C> \<tturnstile> \<Sigma>\<^sub>v \<leadsto>\<^sub>v \<Sigma>\<^sub>v') \<and> \<Sigma>\<^sub>h = unchain_state \<Sigma>\<^sub>v'"
+proof (induction "unchain_state \<Sigma>\<^sub>v" \<Sigma>\<^sub>h arbitrary: \<Sigma>\<^sub>v rule: eval\<^sub>h.induct)
+  case (ev\<^sub>h_lookup \<C> p\<^sub>\<C> x \<Delta>\<^sub>h v h\<^sub>h \<V> s\<^sub>h)
+  then obtain h\<^sub>v \<Delta>\<^sub>v s\<^sub>v' where S: "\<Sigma>\<^sub>v = S\<^sub>v h\<^sub>v \<Delta>\<^sub>v \<V> s\<^sub>v' \<and> h\<^sub>h = unchain_heap h\<^sub>v \<Delta>\<^sub>v \<and> 
+    (\<Delta>\<^sub>h, Suc p\<^sub>\<C>) # s\<^sub>h = unchain_stack \<Delta>\<^sub>v s\<^sub>v'" by fastforce
+  then obtain f\<^sub>v s\<^sub>v where SF: "s\<^sub>v' = f\<^sub>v # s\<^sub>v \<and> (\<Delta>\<^sub>h, Suc p\<^sub>\<C>) = unchain_frame \<Delta>\<^sub>v f\<^sub>v \<and> 
+    s\<^sub>h = unchain_stack \<Delta>\<^sub>v s\<^sub>v" by auto
+  then obtain p\<^sub>\<Delta> where P: "f\<^sub>v = (p\<^sub>\<Delta>, Suc p\<^sub>\<C>) \<and> \<Delta>\<^sub>h = unchain_env \<Delta>\<^sub>v p\<^sub>\<Delta>" by (cases f\<^sub>v) simp_all
+  with ev\<^sub>h_lookup S SF have C: "chain_structured h\<^sub>v \<Delta>\<^sub>v" by simp
+  with ev\<^sub>h_lookup S SF P have X: "S\<^sub>h h\<^sub>h (v # \<V>) ((\<Delta>\<^sub>h, p\<^sub>\<C>) # s\<^sub>h) = 
+    unchain_state (S\<^sub>v h\<^sub>v \<Delta>\<^sub>v (v # \<V>) ((p\<^sub>\<Delta>, p\<^sub>\<C>) # s\<^sub>v))" by simp
+  from ev\<^sub>h_lookup S SF P have "chained_frame \<Delta>\<^sub>v (p\<^sub>\<Delta>, Suc p\<^sub>\<C>)" by simp
+  with C have "lookup (unchain_env \<Delta>\<^sub>v p\<^sub>\<Delta>) x = chain_lookup \<Delta>\<^sub>v p\<^sub>\<Delta> x" by simp
+  with ev\<^sub>h_lookup P C have "\<C> \<tturnstile> S\<^sub>v h\<^sub>v \<Delta>\<^sub>v \<V> ((p\<^sub>\<Delta>, Suc p\<^sub>\<C>) # s\<^sub>v) \<leadsto>\<^sub>v S\<^sub>v h\<^sub>v \<Delta>\<^sub>v (v # \<V>) ((p\<^sub>\<Delta>, p\<^sub>\<C>) # s\<^sub>v)" 
     by simp
-  thus ?case by (simp add: unchain_stack_def)
+  with S SF P X show ?case by blast
 next
-  case (ev\<^sub>v_jump cd pc h v2 p' pc' env v1 env' p'' vs p sfs)
-  from ev\<^sub>v_jump have "chained_closures env h \<and> hcontains h v2" by simp
-  with ev\<^sub>v_jump have "chained_closure env (Lam\<^sub>v p' pc')" by (metis hlookup_all)
-  with ev\<^sub>v_jump have "chain_structured h env \<and> chained_stack_pointer env p' \<and> 
-    halloc env (v1, p') = (env', p'')" by auto
-  hence X: "unstack_list env' (Suc p'') = v1 # unstack_list env p'" by (metis unfold_unstack_list)
-  from ev\<^sub>v_jump have A: "unchain_heap h env' = unchain_heap h env" by auto
-  from ev\<^sub>v_jump have "unchain_stack env' sfs = unchain_stack env sfs" by auto 
-  with ev\<^sub>v_jump X A have "cd \<tturnstile> S\<^sub>h (unchain_heap h env) (v1 # v2 # vs) 
-    ((unstack_list env p, Suc pc) # unchain_stack env sfs) \<leadsto>\<^sub>h
-      S\<^sub>h (unchain_heap h env') vs 
-        ((unstack_list env' (Suc p''), pc') # unchain_stack env' sfs)" by simp
-  thus ?case by (simp add: unchain_stack_def)
-qed (simp_all add: unchain_stack_def)
+  case (ev\<^sub>h_pushcon \<C> p\<^sub>\<C> n h\<^sub>h h\<^sub>h' v \<V> \<Delta>\<^sub>h s\<^sub>h)
+  then obtain h\<^sub>v \<Delta>\<^sub>v s\<^sub>v' where S: "\<Sigma>\<^sub>v = S\<^sub>v h\<^sub>v \<Delta>\<^sub>v \<V> s\<^sub>v' \<and> h\<^sub>h = unchain_heap h\<^sub>v \<Delta>\<^sub>v \<and> 
+    (\<Delta>\<^sub>h, Suc p\<^sub>\<C>) # s\<^sub>h = unchain_stack \<Delta>\<^sub>v s\<^sub>v'" by fastforce
+  then obtain f\<^sub>v s\<^sub>v where SF: "s\<^sub>v' = f\<^sub>v # s\<^sub>v \<and> (\<Delta>\<^sub>h, Suc p\<^sub>\<C>) = unchain_frame \<Delta>\<^sub>v f\<^sub>v \<and> 
+    s\<^sub>h = unchain_stack \<Delta>\<^sub>v s\<^sub>v" by auto
+  then obtain p\<^sub>\<Delta> where P: "f\<^sub>v = (p\<^sub>\<Delta>, Suc p\<^sub>\<C>) \<and> \<Delta>\<^sub>h = unchain_env \<Delta>\<^sub>v p\<^sub>\<Delta>" by (cases f\<^sub>v) simp_all
+  from ev\<^sub>h_pushcon S have "halloc (hmap (unchain_closure \<Delta>\<^sub>v) h\<^sub>v) (unchain_closure \<Delta>\<^sub>v (Const\<^sub>v n)) = 
+    (h\<^sub>h', v)" by simp
+  then obtain h\<^sub>v' where H: "halloc h\<^sub>v (Const\<^sub>v n) = (h\<^sub>v', v) \<and> h\<^sub>h' = hmap (unchain_closure \<Delta>\<^sub>v) h\<^sub>v'" 
+    by (metis halloc_map_inv)
+  hence "h\<^sub>h' = unchain_heap h\<^sub>v' \<Delta>\<^sub>v" by simp
+  with SF P have X: "S\<^sub>h h\<^sub>h' (v # \<V>) ((\<Delta>\<^sub>h, p\<^sub>\<C>) # s\<^sub>h) = 
+    unchain_state (S\<^sub>v h\<^sub>v' \<Delta>\<^sub>v (v # \<V>) ((p\<^sub>\<Delta>, p\<^sub>\<C>) # s\<^sub>v))" by simp
+  from ev\<^sub>h_pushcon H have "\<C> \<tturnstile> S\<^sub>v h\<^sub>v \<Delta>\<^sub>v \<V> ((p\<^sub>\<Delta>, Suc p\<^sub>\<C>) # s\<^sub>v) \<leadsto>\<^sub>v S\<^sub>v h\<^sub>v' \<Delta>\<^sub>v (v # \<V>) ((p\<^sub>\<Delta>, p\<^sub>\<C>) # s\<^sub>v)" 
+    by simp
+  with S SF P X show ?case by blast
+next
+  case (ev\<^sub>h_pushlam \<C> p\<^sub>\<C> p\<^sub>\<C>' h\<^sub>h \<Delta>\<^sub>h h\<^sub>h' v \<V> s\<^sub>h)
+  then obtain h\<^sub>v \<Delta>\<^sub>v s\<^sub>v' where S: "\<Sigma>\<^sub>v = S\<^sub>v h\<^sub>v \<Delta>\<^sub>v \<V> s\<^sub>v' \<and> h\<^sub>h = unchain_heap h\<^sub>v \<Delta>\<^sub>v \<and> 
+    (\<Delta>\<^sub>h, Suc p\<^sub>\<C>) # s\<^sub>h = unchain_stack \<Delta>\<^sub>v s\<^sub>v'" by fastforce
+  then obtain f\<^sub>v s\<^sub>v where SF: "s\<^sub>v' = f\<^sub>v # s\<^sub>v \<and> (\<Delta>\<^sub>h, Suc p\<^sub>\<C>) = unchain_frame \<Delta>\<^sub>v f\<^sub>v \<and> 
+    s\<^sub>h = unchain_stack \<Delta>\<^sub>v s\<^sub>v" by auto
+  then obtain p\<^sub>\<Delta> where P: "f\<^sub>v = (p\<^sub>\<Delta>, Suc p\<^sub>\<C>) \<and> \<Delta>\<^sub>h = unchain_env \<Delta>\<^sub>v p\<^sub>\<Delta>" by (cases f\<^sub>v) simp_all
+  with ev\<^sub>h_pushlam S have "halloc (hmap (unchain_closure \<Delta>\<^sub>v) h\<^sub>v) 
+    (unchain_closure \<Delta>\<^sub>v (Lam\<^sub>v p\<^sub>\<Delta> p\<^sub>\<C>')) = (h\<^sub>h', v)" by simp
+  then obtain h\<^sub>v' where H: "halloc h\<^sub>v (Lam\<^sub>v p\<^sub>\<Delta> p\<^sub>\<C>') = (h\<^sub>v', v) \<and> 
+    h\<^sub>h' = hmap (unchain_closure \<Delta>\<^sub>v) h\<^sub>v'" by (metis halloc_map_inv)
+  hence "h\<^sub>h' = unchain_heap h\<^sub>v' \<Delta>\<^sub>v" by simp
+  with SF P have X: "S\<^sub>h h\<^sub>h' (v # \<V>) ((\<Delta>\<^sub>h, p\<^sub>\<C>) # s\<^sub>h) = 
+    unchain_state (S\<^sub>v h\<^sub>v' \<Delta>\<^sub>v (v # \<V>) ((p\<^sub>\<Delta>, p\<^sub>\<C>) # s\<^sub>v))" by simp
+  from ev\<^sub>h_pushlam H have "\<C> \<tturnstile> S\<^sub>v h\<^sub>v \<Delta>\<^sub>v \<V> ((p\<^sub>\<Delta>, Suc p\<^sub>\<C>) # s\<^sub>v) \<leadsto>\<^sub>v 
+    S\<^sub>v h\<^sub>v' \<Delta>\<^sub>v (v # \<V>) ((p\<^sub>\<Delta>, p\<^sub>\<C>) # s\<^sub>v)" by simp
+  with S SF P X show ?case by blast
+next
+  case (ev\<^sub>h_apply \<C> p\<^sub>\<C> h\<^sub>h v\<^sub>2 \<Delta>\<^sub>h' p\<^sub>\<C>' v\<^sub>1 \<V> \<Delta>\<^sub>h s\<^sub>h)
+  then obtain h\<^sub>v \<Delta>\<^sub>v s\<^sub>v' where S: "\<Sigma>\<^sub>v = S\<^sub>v h\<^sub>v \<Delta>\<^sub>v (v\<^sub>1 # v\<^sub>2 # \<V>) s\<^sub>v' \<and> 
+    h\<^sub>h = unchain_heap h\<^sub>v \<Delta>\<^sub>v \<and> (\<Delta>\<^sub>h, Suc p\<^sub>\<C>) # s\<^sub>h = unchain_stack \<Delta>\<^sub>v s\<^sub>v'" by fastforce
+  then obtain f\<^sub>v s\<^sub>v where SF: "s\<^sub>v' = f\<^sub>v # s\<^sub>v \<and> (\<Delta>\<^sub>h, Suc p\<^sub>\<C>) = unchain_frame \<Delta>\<^sub>v f\<^sub>v \<and> 
+    s\<^sub>h = unchain_stack \<Delta>\<^sub>v s\<^sub>v" by auto
+  then obtain p\<^sub>\<Delta> where P: "f\<^sub>v = (p\<^sub>\<Delta>, Suc p\<^sub>\<C>) \<and> \<Delta>\<^sub>h = unchain_env \<Delta>\<^sub>v p\<^sub>\<Delta>" by (cases f\<^sub>v) simp_all
+  from ev\<^sub>h_apply S have "Lam\<^sub>h \<Delta>\<^sub>h' p\<^sub>\<C>' = unchain_closure \<Delta>\<^sub>v (hlookup h\<^sub>v v\<^sub>2)" by simp
+  then obtain p\<^sub>\<Delta>' where P': "hlookup h\<^sub>v v\<^sub>2 = Lam\<^sub>v p\<^sub>\<Delta>' p\<^sub>\<C>' \<and> \<Delta>\<^sub>h' = unchain_env \<Delta>\<^sub>v p\<^sub>\<Delta>'" by blast
+  obtain \<Delta>\<^sub>v' p\<^sub>\<Delta>'' where H: "halloc \<Delta>\<^sub>v (v\<^sub>1, p\<^sub>\<Delta>') = (\<Delta>\<^sub>v', p\<^sub>\<Delta>'')" 
+    by (cases "halloc \<Delta>\<^sub>v (v\<^sub>1, p\<^sub>\<Delta>')") simp_all
+  from ev\<^sub>h_apply S SF P have C: "chain_structured h\<^sub>v \<Delta>\<^sub>v \<and> chained_closures \<Delta>\<^sub>v h\<^sub>v \<and>
+    hcontains h\<^sub>v v\<^sub>1 \<and> hcontains h\<^sub>v v\<^sub>2 \<and> chained_vals h\<^sub>v \<V> \<and> chained_frame \<Delta>\<^sub>v (p\<^sub>\<Delta>, Suc p\<^sub>\<C>) \<and> 
+      chained_stack \<Delta>\<^sub>v s\<^sub>v" by simp
+  with H have Y: "unchain_heap h\<^sub>v \<Delta>\<^sub>v' = unchain_heap h\<^sub>v \<Delta>\<^sub>v" by fast
+  from H C have "unchain_env \<Delta>\<^sub>v' p\<^sub>\<Delta> = unchain_env \<Delta>\<^sub>v p\<^sub>\<Delta>" by fastforce
+  with P have W: "\<Delta>\<^sub>h = unchain_env \<Delta>\<^sub>v' p\<^sub>\<Delta>" by metis
+  from P' C have "chained_closure \<Delta>\<^sub>v (Lam\<^sub>v p\<^sub>\<Delta>' p\<^sub>\<C>')" by (metis hlookup_all)
+  hence "chained_heap_pointer \<Delta>\<^sub>v p\<^sub>\<Delta>'" by auto
+  with H C have "unchain_env \<Delta>\<^sub>v' (Suc p\<^sub>\<Delta>'') = v\<^sub>1 # unchain_env \<Delta>\<^sub>v p\<^sub>\<Delta>'" 
+    by (metis unfold_unstack_list)
+  with H P' have Z: "v\<^sub>1 # \<Delta>\<^sub>h' = unchain_env \<Delta>\<^sub>v' (Suc p\<^sub>\<Delta>'')" by simp
+  from H C have "unchain_stack \<Delta>\<^sub>v' s\<^sub>v = unchain_stack \<Delta>\<^sub>v s\<^sub>v" by fast
+  with SF have "s\<^sub>h = unchain_stack \<Delta>\<^sub>v' s\<^sub>v" by simp
+  with S Y Z W have X: "S\<^sub>h h\<^sub>h \<V> ((v\<^sub>1 # \<Delta>\<^sub>h', p\<^sub>\<C>') # (\<Delta>\<^sub>h, p\<^sub>\<C>) # s\<^sub>h) = 
+    unchain_state (S\<^sub>v h\<^sub>v \<Delta>\<^sub>v' \<V> ((Suc p\<^sub>\<Delta>'', p\<^sub>\<C>') # (p\<^sub>\<Delta>, p\<^sub>\<C>) # s\<^sub>v))" by simp
+  from ev\<^sub>h_apply P' H have "\<C> \<tturnstile> S\<^sub>v h\<^sub>v \<Delta>\<^sub>v (v\<^sub>1 # v\<^sub>2 # \<V>) ((p\<^sub>\<Delta>, Suc p\<^sub>\<C>) # s\<^sub>v) \<leadsto>\<^sub>v 
+      S\<^sub>v h\<^sub>v \<Delta>\<^sub>v' \<V> ((Suc p\<^sub>\<Delta>'', p\<^sub>\<C>') # (p\<^sub>\<Delta>, p\<^sub>\<C>) # s\<^sub>v)" by simp
+  with S SF P X show ?case by blast
+next
+  case (ev\<^sub>h_return \<C> p\<^sub>\<C> h\<^sub>h \<V> \<Delta>\<^sub>h s\<^sub>h)
+  then obtain h\<^sub>v \<Delta>\<^sub>v s\<^sub>v' where S: "\<Sigma>\<^sub>v = S\<^sub>v h\<^sub>v \<Delta>\<^sub>v \<V> s\<^sub>v' \<and> h\<^sub>h = unchain_heap h\<^sub>v \<Delta>\<^sub>v \<and> 
+    (\<Delta>\<^sub>h, Suc p\<^sub>\<C>) # s\<^sub>h = unchain_stack \<Delta>\<^sub>v s\<^sub>v'" by fastforce
+  then obtain f\<^sub>v s\<^sub>v where SF: "s\<^sub>v' = f\<^sub>v # s\<^sub>v \<and> (\<Delta>\<^sub>h, Suc p\<^sub>\<C>) = unchain_frame \<Delta>\<^sub>v f\<^sub>v \<and> 
+    s\<^sub>h = unchain_stack \<Delta>\<^sub>v s\<^sub>v" by auto
+  then obtain p\<^sub>\<Delta> where P: "f\<^sub>v = (p\<^sub>\<Delta>, Suc p\<^sub>\<C>) \<and> \<Delta>\<^sub>h = unchain_env \<Delta>\<^sub>v p\<^sub>\<Delta>" by (cases f\<^sub>v) simp_all
+  from S SF have X: "S\<^sub>h h\<^sub>h \<V> s\<^sub>h = unchain_state (S\<^sub>v h\<^sub>v \<Delta>\<^sub>v \<V> s\<^sub>v)" by simp
+  from ev\<^sub>h_return have "\<C> \<tturnstile> S\<^sub>v h\<^sub>v \<Delta>\<^sub>v \<V> ((p\<^sub>\<Delta>, Suc p\<^sub>\<C>) # s\<^sub>v) \<leadsto>\<^sub>v S\<^sub>v h\<^sub>v \<Delta>\<^sub>v \<V> s\<^sub>v" by simp
+  with S SF P X show ?case by blast
+next
+  case (ev\<^sub>h_jump \<C> p\<^sub>\<C> h\<^sub>h v\<^sub>2 \<Delta>\<^sub>h' p\<^sub>\<C>' v\<^sub>1 \<V> \<Delta>\<^sub>h s\<^sub>h)
+  then obtain h\<^sub>v \<Delta>\<^sub>v s\<^sub>v' where S: "\<Sigma>\<^sub>v = S\<^sub>v h\<^sub>v \<Delta>\<^sub>v (v\<^sub>1 # v\<^sub>2 # \<V>) s\<^sub>v' \<and> 
+    h\<^sub>h = unchain_heap h\<^sub>v \<Delta>\<^sub>v \<and> (\<Delta>\<^sub>h, Suc p\<^sub>\<C>) # s\<^sub>h = unchain_stack \<Delta>\<^sub>v s\<^sub>v'" by fastforce
+  then obtain f\<^sub>v s\<^sub>v where SF: "s\<^sub>v' = f\<^sub>v # s\<^sub>v \<and> (\<Delta>\<^sub>h, Suc p\<^sub>\<C>) = unchain_frame \<Delta>\<^sub>v f\<^sub>v \<and> 
+    s\<^sub>h = unchain_stack \<Delta>\<^sub>v s\<^sub>v" by auto
+  then obtain p\<^sub>\<Delta> where P: "f\<^sub>v = (p\<^sub>\<Delta>, Suc p\<^sub>\<C>) \<and> \<Delta>\<^sub>h = unchain_env \<Delta>\<^sub>v p\<^sub>\<Delta>" by (cases f\<^sub>v) simp_all
+  from ev\<^sub>h_jump S have "Lam\<^sub>h \<Delta>\<^sub>h' p\<^sub>\<C>' = unchain_closure \<Delta>\<^sub>v (hlookup h\<^sub>v v\<^sub>2)" by simp
+  then obtain p\<^sub>\<Delta>' where P': "hlookup h\<^sub>v v\<^sub>2 = Lam\<^sub>v p\<^sub>\<Delta>' p\<^sub>\<C>' \<and> \<Delta>\<^sub>h' = unchain_env \<Delta>\<^sub>v p\<^sub>\<Delta>'" by blast
+  obtain \<Delta>\<^sub>v' p\<^sub>\<Delta>'' where H: "halloc \<Delta>\<^sub>v (v\<^sub>1, p\<^sub>\<Delta>') = (\<Delta>\<^sub>v', p\<^sub>\<Delta>'')" 
+    by (cases "halloc \<Delta>\<^sub>v (v\<^sub>1, p\<^sub>\<Delta>')") simp_all
+  from ev\<^sub>h_jump S SF P have C: "chain_structured h\<^sub>v \<Delta>\<^sub>v \<and> chained_closures \<Delta>\<^sub>v h\<^sub>v \<and>
+    hcontains h\<^sub>v v\<^sub>1 \<and> hcontains h\<^sub>v v\<^sub>2 \<and> chained_vals h\<^sub>v \<V> \<and> chained_heap_pointer \<Delta>\<^sub>v p\<^sub>\<Delta> \<and> 
+      chained_stack \<Delta>\<^sub>v s\<^sub>v" by simp
+  with H have Y: "unchain_heap h\<^sub>v \<Delta>\<^sub>v' = unchain_heap h\<^sub>v \<Delta>\<^sub>v" by fast
+  from P' C have "chained_closure \<Delta>\<^sub>v (Lam\<^sub>v p\<^sub>\<Delta>' p\<^sub>\<C>')" by (metis hlookup_all)
+  hence "chained_heap_pointer \<Delta>\<^sub>v p\<^sub>\<Delta>'" by simp
+  with H C have "unchain_env \<Delta>\<^sub>v' (Suc p\<^sub>\<Delta>'') = v\<^sub>1 # unchain_env \<Delta>\<^sub>v p\<^sub>\<Delta>'" 
+    by (metis unfold_unstack_list)
+  with H P' have Z: "v\<^sub>1 # \<Delta>\<^sub>h' = unchain_env \<Delta>\<^sub>v' (Suc p\<^sub>\<Delta>'')" by simp
+  from H C have "unchain_stack \<Delta>\<^sub>v' s\<^sub>v = unchain_stack \<Delta>\<^sub>v s\<^sub>v" by fast
+  with SF have "s\<^sub>h = unchain_stack \<Delta>\<^sub>v' s\<^sub>v" by simp
+  with S Y Z have X: "S\<^sub>h h\<^sub>h \<V> ((v\<^sub>1 # \<Delta>\<^sub>h', p\<^sub>\<C>') # s\<^sub>h) = 
+    unchain_state (S\<^sub>v h\<^sub>v \<Delta>\<^sub>v' \<V> ((Suc p\<^sub>\<Delta>'', p\<^sub>\<C>') # s\<^sub>v))" by simp
+  from ev\<^sub>h_jump P' H have "\<C> \<tturnstile> S\<^sub>v h\<^sub>v \<Delta>\<^sub>v (v\<^sub>1 # v\<^sub>2 # \<V>) ((p\<^sub>\<Delta>, Suc p\<^sub>\<C>) # s\<^sub>v) \<leadsto>\<^sub>v 
+      S\<^sub>v h\<^sub>v \<Delta>\<^sub>v' \<V> ((Suc p\<^sub>\<Delta>'', p\<^sub>\<C>') # s\<^sub>v)" by simp
+  with S SF P X show ?case by blast
+qed
 
-lemma [simp]: "halloc env (v, p') = (env', p) \<Longrightarrow> p' < p \<Longrightarrow> hcontains h v \<Longrightarrow> 
-    chain_structured h env \<Longrightarrow> chain_structured h env'"
-  by auto
+text \<open>However, proving that iterated evaluation is correct, which normally has been a trivial 
+corollary, turns out to require a bit more machinery; the \<open>chained_state\<close> property is preserved by 
+evaluation, but showing this (\<open>eval_preserves_chained\<close>) takes a few more lemmas, mostly dealing with
+allocating into the environment heap.\<close>
 
-lemma [simp]: "halloc env v = (env', p) \<Longrightarrow> chained_stack_pointer env a \<Longrightarrow> 
-    chained_stack_pointer env' a"
-  by (cases a) simp_all
+lemma halloc_chained_heap_pointer [simp]: "halloc \<Delta> v = (\<Delta>', p) \<Longrightarrow> chained_heap_pointer \<Delta> x \<Longrightarrow> 
+    chained_heap_pointer \<Delta>' x"
+  by (cases x) simp_all
 
-lemma [simp]: "halloc env (v, p') = (env', p) \<Longrightarrow> chained_frame env f \<Longrightarrow> chained_frame env' f"
+lemma hallock_chained_closure [simp]: "halloc \<Delta> v = (\<Delta>', p) \<Longrightarrow> chained_closure \<Delta> c \<Longrightarrow> 
+    chained_closure \<Delta>' c"
+  by (induction c) simp_all
+
+lemma hallock_chained_closures [simp]: "halloc \<Delta> v = (\<Delta>', p) \<Longrightarrow> chained_closures \<Delta> h \<Longrightarrow> 
+  chained_closures \<Delta>' h"
+proof -
+  assume "halloc \<Delta> v = (\<Delta>', p)"
+  hence "\<And>y. chained_closure \<Delta> y \<Longrightarrow> chained_closure \<Delta>' y" by simp_all
+  moreover assume "chained_closures \<Delta> h"
+  ultimately show "chained_closures \<Delta>' h" by (metis heap_all_implication)
+qed
+
+lemma halloc_chained_frame [simp]: "halloc \<Delta> (v, p') = (\<Delta>', p) \<Longrightarrow> chained_frame \<Delta> f \<Longrightarrow> 
+    chained_frame \<Delta>' f"
   by (induction f) simp_all
 
-lemma [simp]: "halloc env (v, p') = (env', p) \<Longrightarrow> chained_stack env sfs \<Longrightarrow> 
-    chained_stack env' sfs"
-  by (induction sfs) simp_all
+lemma hallock_chained_stack [simp]: "halloc \<Delta> (v, p') = (\<Delta>', p) \<Longrightarrow> chained_stack \<Delta> s \<Longrightarrow> 
+    chained_stack \<Delta>' s"
+  by (induction s) simp_all
 
-lemma [elim]: "chain_structured h env \<Longrightarrow> hcontains env p \<Longrightarrow> hlookup env p = (a, b) \<Longrightarrow> 
-    hcontains h a"
+lemma chained_hlookup_hcontains [elim]: "chain_structured h \<Delta> \<Longrightarrow> hcontains \<Delta> p \<Longrightarrow> 
+  hlookup \<Delta> p = (a, b) \<Longrightarrow> hcontains h a"
 proof -
-  assume "chain_structured h env" and "hcontains env p" and "hlookup env p = (a, b)"
+  assume "chain_structured h \<Delta>" and "hcontains \<Delta> p" and "hlookup \<Delta> p = (a, b)"
   hence "(\<lambda>(v, p'). p' \<le> p \<and> hcontains h v) (a, b)" by (metis hlookup_all)
   thus ?thesis by simp
 qed
 
-lemma [elim]: "chain_structured h env \<Longrightarrow> hcontains env p \<Longrightarrow> chain_lookup env p x = Some v \<Longrightarrow> 
-  hcontains h v"
-proof (induction env p x rule: chain_lookup.induct)
-  case (2 env p)
-  moreover obtain a b where "hlookup env p = (a, b)" by (cases "hlookup env p")
+lemma chain_lookup_hcontains [elim]: "chain_structured h \<Delta> \<Longrightarrow> hcontains \<Delta> p \<Longrightarrow> 
+  chain_lookup \<Delta> p x = Some v \<Longrightarrow> hcontains h v"
+proof (induction \<Delta> p x rule: chain_lookup.induct)
+  case (2 \<Delta> p)
+  moreover obtain a b where "hlookup \<Delta> p = (a, b)" by (cases "hlookup \<Delta> p")
   ultimately show ?case by auto
 next
-  case (3 env p x)
-  obtain a b where A: "hlookup env p = (a, b)" by (cases "hlookup env p")
-  from 3 have "hcontains env p" by auto
+  case (3 \<Delta> p x)
+  obtain a b where A: "hlookup \<Delta> p = (a, b)" by (cases "hlookup \<Delta> p")
+  from 3 have "hcontains \<Delta> p" by auto
   with 3 A have "b \<le> p \<and> hcontains h a" using hlookup_all by fast
-  with 3 have "hcontains env b" by fastforce
+  with 3 have "hcontains \<Delta> b" by fastforce
   with 3 A show ?case by simp
 qed simp_all
 
-lemma [simp]: "halloc h v = (h', p) \<Longrightarrow> chain_structured h env \<Longrightarrow> chain_structured h' env"
-proof -
-  define pp where "pp = (\<lambda>(p::nat) (v, p'). p' \<le> p \<and> hcontains h v)"
-  define qq where "qq = (\<lambda>(p::nat) (v, p'). p' \<le> p \<and> hcontains h' v)"
-  assume "halloc h v = (h', p)"
-  hence A: "\<And>x y. pp x y \<Longrightarrow> qq x y" by (auto simp add: pp_def qq_def split: prod.splits)
-  assume "chain_structured h env"
-  hence "heap_all pp env" by (simp add: pp_def)
-  with A have "heap_all qq env" by (metis heap_all_implication)
-  thus "chain_structured h' env" by (simp add: qq_def)
+lemma chain_lookup_suc_hcontains [elim]: "chain_lookup \<Delta> (Suc p) x = Some v \<Longrightarrow> 
+  chain_structured h \<Delta> \<Longrightarrow> hcontains \<Delta> p \<Longrightarrow> hcontains h v"
+proof (induction \<Delta> "Suc p" x arbitrary: p rule: chain_lookup.induct)
+  case (2 \<Delta> p)
+  then obtain b where "hlookup \<Delta> p = (v, b)" by (cases "hlookup \<Delta> p") simp_all
+  with 2 have "b \<le> p \<and> hcontains h v" using hlookup_all by fast
+  with 2 show ?case by simp
+next
+  case (3 \<Delta> p x)
+  moreover then obtain a b where A: "hlookup \<Delta> p = (a, b)" by (cases "hlookup \<Delta> p")
+  moreover with 3 have "b \<le> p \<and> hcontains h a" using hlookup_all by fast
+  ultimately show ?case by auto
 qed
 
-lemma [simp]: "halloc h v = (h', p) \<Longrightarrow> chained_vals h vs \<Longrightarrow> chained_vals h' vs"
-  by (induction vs) auto
-
-lemma [simp]: "halloc env v = (env', p) \<Longrightarrow> chained_closure env c \<Longrightarrow> chained_closure env' c"
-  by (induction c) simp_all
-
-lemma [simp]: "halloc env v = (env', p) \<Longrightarrow> chained_closures env h \<Longrightarrow> chained_closures env' h"
+lemma chain_structured_alloc_lam [simp]: "hcontains h v\<^sub>2 \<Longrightarrow> hlookup h v\<^sub>2 = Lam\<^sub>v p\<^sub>\<Delta> p\<^sub>\<C> \<Longrightarrow> 
+  chained_closures \<Delta> h \<Longrightarrow> hcontains h v\<^sub>1 \<Longrightarrow> halloc \<Delta> (v\<^sub>1, p\<^sub>\<Delta>) = (\<Delta>', p\<^sub>\<Delta>') \<Longrightarrow> 
+    chain_structured h \<Delta> \<Longrightarrow> chain_structured h \<Delta>'"
 proof -
-  assume "halloc env v = (env', p)"
-  hence "\<And>y. chained_closure env y \<Longrightarrow> chained_closure env' y" by simp_all
-  moreover assume "chained_closures env h"
-  ultimately show "chained_closures env' h" by (metis heap_all_implication)
-qed
-
-lemma [simp]: "hlookup h v2 = Lam\<^sub>v p' pc' \<Longrightarrow> chained_closures env h \<Longrightarrow> hcontains h v2 \<Longrightarrow> 
-  hcontains h v1 \<Longrightarrow> halloc env (v1, p') = (env', p'') \<Longrightarrow> chain_structured h env \<Longrightarrow> 
-    chain_structured h env'"
-proof -
-  assume "chained_closures env h" and "hlookup h v2 = Lam\<^sub>v p' pc'" and "hcontains h v2"
-  hence X: "chained_stack_pointer env p'" using hlookup_all by fastforce
-  moreover assume A: "halloc env (v1, p') = (env', p'')" and "chain_structured h env" 
-    and "hcontains h v1"
-  moreover have "p' \<le> p''"
-  proof (cases p')
+  assume "chained_closures \<Delta> h" and "hlookup h v\<^sub>2 = Lam\<^sub>v p\<^sub>\<Delta> p\<^sub>\<C>" and "hcontains h v\<^sub>2"
+  hence X: "chained_heap_pointer \<Delta> p\<^sub>\<Delta>" using hlookup_all by fastforce
+  moreover assume A: "halloc \<Delta> (v\<^sub>1, p\<^sub>\<Delta>) = (\<Delta>', p\<^sub>\<Delta>')" and "chain_structured h \<Delta>" 
+    and "hcontains h v\<^sub>1"
+  moreover have "p\<^sub>\<Delta> \<le> p\<^sub>\<Delta>'"
+  proof (cases p\<^sub>\<Delta>)
     case (Suc pp)
-    moreover with X A have "pp < p''" by simp
+    moreover with X A have "pp < p\<^sub>\<Delta>'" by simp
     ultimately show ?thesis by simp
   qed simp_all
   ultimately show ?thesis by auto
 qed
 
-lemma [elim]: "chain_lookup env (Suc p) x = Some v \<Longrightarrow> chain_structured h env \<Longrightarrow> 
-  hcontains env p \<Longrightarrow> hcontains h v"
-proof (induction env "Suc p" x arbitrary: p rule: chain_lookup.induct)
-  case (2 env p)
-  then obtain b where "hlookup env p = (v, b)" by (cases "hlookup env p") simp_all
-  with 2 have "b \<le> p \<and> hcontains h v" using hlookup_all by fast
-  with 2 show ?case by simp
-next
-  case (3 env p x)
-  moreover then obtain a b where A: "hlookup env p = (a, b)" by (cases "hlookup env p")
-  moreover with 3 have "b \<le> p \<and> hcontains h a" using hlookup_all by fast
-  ultimately show ?case by auto
+lemma chain_structured_unfold [simp]: "chain_structured h \<Delta> \<Longrightarrow> 
+  heap_all (\<lambda>p (y, p'). p' \<le> p \<and> (y = x \<or> hcontains h y)) \<Delta>"
+proof -
+  have "\<And>a b. (\<lambda>p (v, p'). p' \<le> p \<and> hcontains h v) a b \<Longrightarrow> 
+    (\<lambda>p (y, p'). p' \<le> p \<and> (y = x \<or> hcontains h y)) a b" by (simp split: prod.splits)
+  moreover assume "chain_structured h \<Delta>"
+  ultimately show "heap_all (\<lambda>p (y, p'). p' \<le> p \<and> (y = x \<or> hcontains h y)) \<Delta>"
+    by (rule heap_all_implication)
 qed
 
-lemma [simp]: "cd \<tturnstile> \<Sigma>\<^sub>c\<^sub>e \<leadsto>\<^sub>v \<Sigma>\<^sub>c\<^sub>e' \<Longrightarrow> chained_state \<Sigma>\<^sub>c\<^sub>e \<Longrightarrow> chained_state \<Sigma>\<^sub>c\<^sub>e'"
-proof (induction \<Sigma>\<^sub>c\<^sub>e \<Sigma>\<^sub>c\<^sub>e' rule: eval\<^sub>v.induct)
-  case (ev\<^sub>v_lookup cd pc x env p v h vs sfs)
+lemma eval_preserves_chained [simp]: "\<C> \<tturnstile> \<Sigma>\<^sub>v \<leadsto>\<^sub>v \<Sigma>\<^sub>v' \<Longrightarrow> chained_state \<Sigma>\<^sub>v \<Longrightarrow> chained_state \<Sigma>\<^sub>v'"
+proof (induction \<Sigma>\<^sub>v \<Sigma>\<^sub>v' rule: eval\<^sub>v.induct)
+  case (ev\<^sub>v_lookup \<C> p\<^sub>\<C> x \<Delta> p v h \<V> s)
   thus ?case by (cases p) auto
 qed auto
 
-lemma [simp]: "iter (\<tturnstile> cd \<leadsto>\<^sub>v) \<Sigma>\<^sub>c\<^sub>e \<Sigma>\<^sub>c\<^sub>e' \<Longrightarrow> chained_state \<Sigma>\<^sub>c\<^sub>e \<Longrightarrow> 
-  iter (\<tturnstile> cd \<leadsto>\<^sub>h) (unchain_state \<Sigma>\<^sub>c\<^sub>e) (unchain_state \<Sigma>\<^sub>c\<^sub>e')"
-proof (induction \<Sigma>\<^sub>c\<^sub>e \<Sigma>\<^sub>c\<^sub>e' rule: iter.induct)
-  case (iter_step \<Sigma>\<^sub>c\<^sub>e \<Sigma>\<^sub>c\<^sub>e' \<Sigma>\<^sub>c\<^sub>e'')
-  hence "iter (\<tturnstile> cd \<leadsto>\<^sub>h) (unchain_state \<Sigma>\<^sub>c\<^sub>e') (unchain_state \<Sigma>\<^sub>c\<^sub>e'')" by simp
-  moreover from iter_step have "cd \<tturnstile> unchain_state \<Sigma>\<^sub>c\<^sub>e \<leadsto>\<^sub>h unchain_state \<Sigma>\<^sub>c\<^sub>e'" by simp
-  ultimately show ?case by simp
-qed simp_all
+lemma preserve_chained [simp]: "iter (\<tturnstile> \<C> \<leadsto>\<^sub>v) \<Sigma>\<^sub>v \<Sigma>\<^sub>v' \<Longrightarrow> chained_state \<Sigma>\<^sub>v \<Longrightarrow> chained_state \<Sigma>\<^sub>v'"
+  by (induction \<Sigma>\<^sub>v \<Sigma>\<^sub>v' rule: iter.induct) simp_all
 
-lemma [simp]: "iter (\<tturnstile> cd \<leadsto>\<^sub>h) (unchain_state \<Sigma>\<^sub>c\<^sub>e) \<Sigma>\<^sub>h \<Longrightarrow> chained_state \<Sigma>\<^sub>c\<^sub>e \<Longrightarrow> 
-  \<exists>\<Sigma>\<^sub>c\<^sub>e'. iter (\<tturnstile> cd \<leadsto>\<^sub>v) \<Sigma>\<^sub>c\<^sub>e \<Sigma>\<^sub>c\<^sub>e' \<and> \<Sigma>\<^sub>h = unchain_state \<Sigma>\<^sub>c\<^sub>e'"
-proof (induction "unchain_state \<Sigma>\<^sub>c\<^sub>e" \<Sigma>\<^sub>h arbitrary: \<Sigma>\<^sub>c\<^sub>e rule: iter.induct)
+lemma correct\<^sub>v_iter [simp]: "iter (\<tturnstile> \<C> \<leadsto>\<^sub>h) (unchain_state \<Sigma>\<^sub>v) \<Sigma>\<^sub>h \<Longrightarrow> chained_state \<Sigma>\<^sub>v \<Longrightarrow> 
+  \<exists>\<Sigma>\<^sub>v'. iter (\<tturnstile> \<C> \<leadsto>\<^sub>v) \<Sigma>\<^sub>v \<Sigma>\<^sub>v' \<and> \<Sigma>\<^sub>h = unchain_state \<Sigma>\<^sub>v'"
+proof (induction "unchain_state \<Sigma>\<^sub>v" \<Sigma>\<^sub>h arbitrary: \<Sigma>\<^sub>v rule: iter.induct)
   case (iter_step \<Sigma>\<^sub>h' \<Sigma>\<^sub>h'')
-  then obtain \<Sigma>\<^sub>c\<^sub>e' where "(cd \<tturnstile> \<Sigma>\<^sub>c\<^sub>e \<leadsto>\<^sub>v \<Sigma>\<^sub>c\<^sub>e') \<and> \<Sigma>\<^sub>h' = unchain_state \<Sigma>\<^sub>c\<^sub>e'" by fastforce
-  moreover with iter_step obtain \<Sigma>\<^sub>c\<^sub>e'' where "iter (\<tturnstile> cd \<leadsto>\<^sub>v) \<Sigma>\<^sub>c\<^sub>e' \<Sigma>\<^sub>c\<^sub>e'' \<and> 
-    \<Sigma>\<^sub>h'' = unchain_state \<Sigma>\<^sub>c\<^sub>e''" by fastforce
-  ultimately have "iter (\<tturnstile> cd \<leadsto>\<^sub>v) \<Sigma>\<^sub>c\<^sub>e \<Sigma>\<^sub>c\<^sub>e'' \<and> \<Sigma>\<^sub>h'' = unchain_state \<Sigma>\<^sub>c\<^sub>e''" by fastforce
+  moreover then obtain \<Sigma>\<^sub>v' where S: "(\<C> \<tturnstile> \<Sigma>\<^sub>v \<leadsto>\<^sub>v \<Sigma>\<^sub>v') \<and> \<Sigma>\<^sub>h' = unchain_state \<Sigma>\<^sub>v'" by fastforce
+  moreover with iter_step have "chained_state \<Sigma>\<^sub>v'" by (metis eval_preserves_chained)
+  ultimately obtain \<Sigma>\<^sub>v'' where "iter (\<tturnstile> \<C> \<leadsto>\<^sub>v) \<Sigma>\<^sub>v' \<Sigma>\<^sub>v'' \<and> \<Sigma>\<^sub>h'' = unchain_state \<Sigma>\<^sub>v''" by blast
+  with S have "iter (\<tturnstile> \<C> \<leadsto>\<^sub>v) \<Sigma>\<^sub>v \<Sigma>\<^sub>v'' \<and> \<Sigma>\<^sub>h'' = unchain_state \<Sigma>\<^sub>v''" by fastforce
   then show ?case by fastforce
 qed force+
-
-lemma preserve_chained [simp]: "iter (\<tturnstile> cd \<leadsto>\<^sub>v) \<Sigma>\<^sub>c\<^sub>e \<Sigma>\<^sub>c\<^sub>e' \<Longrightarrow> chained_state \<Sigma>\<^sub>c\<^sub>e \<Longrightarrow> 
-    chained_state \<Sigma>\<^sub>c\<^sub>e'"
-  by (induction \<Sigma>\<^sub>c\<^sub>e \<Sigma>\<^sub>c\<^sub>e' rule: iter.induct) simp_all
 
 end
